Stratego/Stratego.thy
@@ -23,7 +23,7 @@ using the @{term Rewritable} class.
   by simp+
 
 termination n*)
-
+  
 class Rewritable = size +
   fixes rewrite :: "('a \<Rightarrow> 'a) \<Rightarrow> 'a \<Rightarrow> 'a"
   fixes match :: "'a \<Rightarrow> 'a \<Rightarrow> ((string, 'a) fmap) option"
@@ -31,16 +31,21 @@ class Rewritable = size +
   fixes var :: "string \<Rightarrow> 'a"
   fixes subexprs :: "'a \<Rightarrow> 'a list"
   (*fixes map :: "('a \<Rightarrow> 'a) \<Rightarrow> 'a \<Rightarrow> 'a"*)
-  fixes chain :: "nat \<Rightarrow> ('a \<Rightarrow> nat \<Rightarrow> (nat \<times> 'a)) \<Rightarrow> 'a \<Rightarrow> (nat \<times> 'a)"
+  fixes chain :: "('a \<Rightarrow> nat \<Rightarrow> (nat \<times> 'a)) \<Rightarrow> 'a \<Rightarrow> nat \<Rightarrow> (nat \<times> 'a)"
   (*assumes "varof (var a) = Some a"
   assumes "traverse f t = traverse f (traverse f t)"*)
   assumes shrinks: "\<forall>e' \<in> set (subexprs e). size e > size e'"
-  assumes "map f (subexprs e) = subexprs (snd (chain 0 (\<lambda>e a. (plus a 1, f e)) e))"
-  assumes "length (subexprs e) = fst (chain 0 (\<lambda>e a. (plus a 1, f e)) e)"
+  assumes "map f (subexprs e) = subexprs (snd (chain (\<lambda>e a. (plus a 1, f e)) e 0))"
+  assumes "length (subexprs e) = fst (chain (\<lambda>e a. (plus a 1, f e)) e 0)"
   (*assumes chain_term: "All chain_dom"*)
 begin
 fun map_tree :: "('a \<Rightarrow> 'a) \<Rightarrow> 'a \<Rightarrow> 'a" where
-  "map_tree f xs = snd (chain (0::nat) (\<lambda>e a. (plus a 1, f e)) xs)"
+  "map_tree f xs = snd (chain (\<lambda>e a. (plus a 1, f e)) xs (0::nat))"
+
+fun maybe_map_tree :: "('a \<Rightarrow> 'a option) \<Rightarrow> 'a \<Rightarrow> 'a option" where
+  "maybe_map_tree f xs = 
+    (let (flag, e') = (chain (\<lambda>e a. (if (f e) = None then 1 else 0, the (f e))) xs (0::nat)) in
+      (if flag = 1 then None else Some e'))"
 
 fun pattern_variables :: "'a \<Rightarrow> string list" where
   "pattern_variables e = List.map_filter varof (subexprs e)"
@@ -58,7 +63,6 @@ fun chain_list :: "'b \<Rightarrow> ('a \<Rightarrow> 'b \<Rightarrow> ('b \<tim
     (let (a'', xs') = (chain_list a' f xs) in (a'', x' # xs')))"
 
 
-
 subsection "Rewrite Language"
 datatype ('a::Rewritable) Strategy =
   id | \<comment> \<open>identity operator\<close>
@@ -66,44 +70,46 @@ datatype ('a::Rewritable) Strategy =
   func "'a \<Rightarrow> 'a" | \<comment> \<open>apply an arbitrary function transformation to the subject\<close>
   ematch 'a ("_?" [121] 120) | \<comment> \<open>match the subject to the given Rewritable, updating the binding\<close>
   promote 'a ("_!" [121] 120) | \<comment> \<open>ground and promote the given Rewritable to the subject\<close>
-  condition "'a Strategy" "'a Strategy" "'a Strategy" ("_ < _ + _" 105) \<comment> \<open>if the first strategy succeeds, apply the second, else the third\<close>
+  condition "('a) Strategy" "('a) Strategy" "('a) Strategy" ("_ < _ + _" 105) \<comment> \<open>if the first strategy succeeds, apply the second, else the third\<close>
 
 subsubsection "Language Extensions"
 
-abbreviation seq :: "'a::Rewritable Strategy \<Rightarrow> 'a Strategy \<Rightarrow> 'a Strategy"
+abbreviation seq :: "('a::Rewritable) Strategy \<Rightarrow> ('a) Strategy \<Rightarrow> ('a) Strategy"
   (infixl ";" 110) where
   "s1; s2 \<equiv> s1 < s2 + fail"
 
-abbreviation else :: "'a::Rewritable Strategy \<Rightarrow> 'a Strategy \<Rightarrow> 'a Strategy"
+abbreviation else :: "('a::Rewritable) Strategy \<Rightarrow> ('a) Strategy \<Rightarrow> ('a) Strategy"
   ("_ <+ _" 111) where
   "s1 <+ s2 \<equiv> s1 < id + s2"
 
-abbreviation rewrite_to :: "'a::Rewritable \<Rightarrow> 'a \<Rightarrow> 'a Strategy"
+abbreviation rewrite_to :: "'a::Rewritable \<Rightarrow> 'a \<Rightarrow> ('a) Strategy"
   ("_ \<rightarrow> _") where
   "(s1 \<rightarrow> s2) \<equiv> s1?; s2!"
 
-abbreviation "wheref" :: "('a::Rewritable) Strategy \<Rightarrow> 'a Strategy" where
+abbreviation "wheref" :: "('a::Rewritable) Strategy \<Rightarrow> ('a) Strategy" where
   "wheref x \<equiv> var ''_''?; x; var ''_''!"
 
-abbreviation conditional_rewrite_to :: "'a::Rewritable \<Rightarrow> 'a \<Rightarrow> 'a Strategy \<Rightarrow> 'a Strategy"
+abbreviation conditional_rewrite_to :: "'a::Rewritable \<Rightarrow> 'a \<Rightarrow> ('a) Strategy \<Rightarrow> ('a) Strategy"
   ("_ \<rightarrow> _ where _") where 
   "s1 \<rightarrow> s2 where s3 \<equiv> s1?; wheref s3; s2!"
 
-definition not :: "('a::Rewritable) Strategy \<Rightarrow> 'a Strategy" where 
+definition not :: "('a::Rewritable) Strategy \<Rightarrow> ('a) Strategy" where 
   "not s = (s < fail + id)"
 
-abbreviation "apply" :: "(('a::Rewritable) \<Rightarrow> 'a) \<Rightarrow> 'a \<Rightarrow> 'a Strategy" 
+abbreviation "apply" :: "('a \<Rightarrow> 'a) \<Rightarrow> 'a \<Rightarrow> ('a::Rewritable) Strategy" 
   ("<_>(_)") where
   "(<f>(vars)) \<equiv> vars!; func f"
 
 fun wrap_pred :: "(('a::Rewritable) \<Rightarrow> bool) \<Rightarrow> ('a \<Rightarrow> 'a)" where
   "wrap_pred f = (\<lambda>t. if f t then var ''true'' else var ''false'')"
 
+(*
 abbreviation "pred" :: "(('a::Rewritable) \<Rightarrow> bool) \<Rightarrow> 'a \<Rightarrow> 'a Strategy" 
   ("<_>?(_)") where
   "(<f>?(vars)) \<equiv> vars!; func (wrap_pred f); var ''true''?"
+*)
 
-abbreviation assign :: "('a::Rewritable) \<Rightarrow> 'a Strategy \<Rightarrow> 'a Strategy" 
+abbreviation assign :: "'a::Rewritable \<Rightarrow> ('a) Strategy \<Rightarrow> ('a) Strategy" 
   ("_ := _") where 
   \<comment> \<open>This should be trm => vars but this doesn't work well in Isabelle so swapped argument order.\<close>
   "vars := trm \<equiv> trm; vars?"
@@ -122,7 +128,7 @@ fun ground :: "('a::Rewritable) Binding \<Rightarrow> 'a \<Rightarrow> 'a" where
 fun substitute :: "('a::Rewritable) Binding \<Rightarrow> 'a \<Rightarrow> 'a" where
   "substitute b trm = rewrite (ground b) trm"
 
-fun eval :: "'a Strategy \<Rightarrow> ('a::Rewritable) State \<Rightarrow> ('a State \<times> bool)" where
+fun eval :: "('a) Strategy \<Rightarrow> ('a::Rewritable) State \<Rightarrow> ('a State \<times> bool)" where
   "eval (s!) (sub, b) = ((substitute b s, b), True)" |
   "eval (s?) (sub, b) =
       (case match s sub of
@@ -194,20 +200,20 @@ fun subexprs_Arithmetic :: "Arithmetic \<Rightarrow> Arithmetic list" where
   "subexprs_Arithmetic (Number v) = []" |
   "subexprs_Arithmetic (Variable s) = []"
 
-fun chain_Arithmetic :: "nat \<Rightarrow> (Arithmetic \<Rightarrow> nat \<Rightarrow> (nat \<times> Arithmetic)) \<Rightarrow> Arithmetic \<Rightarrow> (nat \<times> Arithmetic)" where
-  "chain_Arithmetic n f (Add x y) =
+fun chain_Arithmetic :: "(Arithmetic \<Rightarrow> nat \<Rightarrow> (nat \<times> Arithmetic)) \<Rightarrow> Arithmetic \<Rightarrow> nat \<Rightarrow> (nat \<times> Arithmetic)" where
+  "chain_Arithmetic f (Add x y) n =
     (let (n', x') = f x n in
     (let (n'', y') = f y n' in
       (n'', Add x' y')))" |
-  "chain_Arithmetic n f (Sub x y) =
+  "chain_Arithmetic f (Sub x y) n =
     (let (n', x') = f x n in
     (let (n'', y') = f y n' in
       (n'', Sub x' y')))" |
-  "chain_Arithmetic n f (UMinus x) =
+  "chain_Arithmetic f (UMinus x) n =
     (let (n', x') = f x n in
       (n', UMinus x'))" |
-  "chain_Arithmetic n f (Number v) = (n, (Number v))" |
-  "chain_Arithmetic n f (Variable s) = (n, (Variable s))"
+  "chain_Arithmetic f (Number v) n = (n, (Number v))" |
+  "chain_Arithmetic f (Variable s) n = (n, (Variable s))"
 
 (*
 fun map_Arithmetic where
@@ -225,36 +231,61 @@ instance proof
 next
   fix f :: "Arithmetic \<Rightarrow> Arithmetic"
   fix e :: Arithmetic
-  show "map f (subexprs e) = subexprs (snd (chain 0 (\<lambda>e a. (plus a 1, f e)) e))"
+  show "map f (subexprs e) = subexprs (snd (chain (\<lambda>e a. (plus a 1, f e)) e 0))"
     by (cases e; simp)
 next
   fix f :: "Arithmetic \<Rightarrow> Arithmetic"
   fix e :: Arithmetic
-  show "length (subexprs e) = fst (chain 0 (\<lambda>e a. (plus a 1, f e)) e)"
+  show "length (subexprs e) = fst (chain (\<lambda>e a. (plus a 1, f e)) e 0)"
     by (cases e; simp)
 qed
 end
 
+(*
+datatype ArithmeticCondition =
+  IsSub Arithmetic |
+  IsNumber Arithmetic
 
+instantiation ArithmeticCondition :: Condition begin
+fun eval_condition_ArithmeticCondition :: "ArithmeticCondition \<Rightarrow> bool" where
+  "eval_condition_ArithmeticCondition (IsSub (Sub x y)) = True" |
+  "eval_condition_ArithmeticCondition (IsNumber (Number v)) = True" |
+  "eval_condition_ArithmeticCondition _ = False"
+
+fun ground_condition_ArithmeticCondition :: "ArithmeticCondition \<Rightarrow> (string \<Rightarrow> string) \<Rightarrow> ArithmeticCondition" where
+  "ground_condition_ArithmeticCondition (IsSub (Variable v)) f = (IsSub (var (f v)))" |
+  "ground_condition_ArithmeticCondition (IsNumber (Variable v)) f = (IsNumber (var (f v)))" |
+  "ground_condition_ArithmeticCondition e f = e"
+
+instance proof qed
+end
+*)
 
 subsubsection "Rewrite Rules"
 
-definition RedundantAdd :: "Arithmetic Strategy" where
-  "RedundantAdd = ((Add (Variable ''a'') (Number (0::int))) \<rightarrow> (Variable ''a''))"
+definition RedundantAdd :: "(Arithmetic) Strategy" where
+  "RedundantAdd = ((Add (var ''b'') (Number 0)) \<rightarrow> (var ''b''))"
 
-definition RedundantSub :: "Arithmetic Strategy" where
-  "RedundantSub = ((Sub (Variable ''a'') (Number (0::int))) \<rightarrow> (Variable ''a''))"
+definition RedundantSub :: "(Arithmetic) Strategy" where
+  "RedundantSub = ((Sub (var ''a'') (Number 0)) \<rightarrow> (var ''a''))"
 
-definition ShiftConstRight :: "Arithmetic Strategy" where
+definition ShiftConstRight :: "(Arithmetic) Strategy" where
   "ShiftConstRight = 
-    ((Add (Variable ''a'') (Variable ''b'')) \<rightarrow> (Add (Variable ''b'') (Variable ''a''))
-      where ((Variable ''a'')!; not (Number 0?)))"
+    ((Add (var ''a'') (var ''b'')) \<rightarrow> (Add (var ''b'') (var ''a''))
+      where ((var ''a'')!; not (Number 0?)))"
+
+
+(*definition ShiftConstRight2 :: "(Arithmetic) Strategy" where
+  "ShiftConstRight2 = 
+    ((Add (var ''a'') (var ''b'')) \<rightarrow> (Add (var ''b'') (var ''a''))
+      where ((var ''a'')!; func is_Number))"*)
 
 fun negate :: "Arithmetic \<Rightarrow> Arithmetic" where
   "negate (Number v) = (Number (-v))" |
   "negate x = x"
 
-definition EvalMinus :: "Arithmetic Strategy" where
+(*
+definition EvalMinus :: "(Arithmetic) Strategy" where
   "EvalMinus = 
     ((UMinus (Variable ''a'')) \<rightarrow> ((Variable ''b''))
       where (<is_Number>?(Variable ''a''); ((Variable ''a'')!; func negate); (Variable ''b'')?))"
@@ -276,6 +307,7 @@ definition EvalAdd :: "Arithmetic Strategy" where
         <is_Number>?(Variable ''b'');
         (Variable ''c'') := <add>(Add (Variable ''a'') (Variable ''b''))
       )"
+*)
 
 subsubsection "Rewrite Application"
 
@@ -303,6 +335,10 @@ value "ShiftConstRight"
 value "eval ShiftConstRight ((Add (Number 0) (Number 10)), fmempty)"
 value "eval ShiftConstRight ((Add (Number 10) (Add (Number 10) (Number 20))), fmempty)"
 value "eval ShiftConstRight ((Add (Number 10) (Number 10)), fmempty)"
+
+value "eval ShiftConstRight2 ((Add (Number 0) (Number 10)), fmempty)"
+value "eval ShiftConstRight2 ((Add (Number 10) (Add (Number 10) (Number 20))), fmempty)"
+value "eval ShiftConstRight2 ((Add (Number 10) (Number 10)), fmempty)"
 
 value "eval EvalMinus ((UMinus (Number 10)), fmempty)"
 value "eval EvalMinus ((UMinus (Add (Number 10) (Number 10))), fmempty)"
