VeriComp/Optimizations.thy
@@ -1,0 +1,13 @@
+theory Optimizations
+  imports
+    Optimizations.Canonicalizations.Common
+    Proofs.StampEvalThms
+begin
+
+phase ConditionalNode
+  terminating size
+begin
+
+end
+
+end
